\documentclass[a4paper]{scrartcl}
\input{../header.tex}

\subject{Funktionale Programmierung WS 2013/14}
\title{Ãœbungsblatt 3}
\author{Kevin Dungs\thanks{kevin.dungs@udo.edu}}

\begin{document}
\maketitle

\section*{Aufgabe 3.1}
\paragraph{1)}
\begin{minted}{haskell}
    Int -> (Bool, a) -> (a, Int)
  = (Int -> (Bool, a)) -> (a, Int)
\end{minted}

\paragraph{2)}
\begin{minted}{haskell}
    Int -> Bool -> (Int, Int) -> Int
  = ((Int -> Bool) -> (Int, Int)) -> Int
\end{minted}

\paragraph{3)}
\begin{minted}{haskell}
    a -> (a -> b -> c) -> b -> a
  = ((a -> ((a -> b) -> c)) -> b) -> a
\end{minted}


\section*{Aufgabe 3.2}
\paragraph{1)}
\begin{minted}{haskell}
    (\f -> f . f) $ \x -> (+3) x
  = \x -> ((+3) . (+3)) x
  = x + 6
\end{minted}

\paragraph{2)}
\begin{minted}{haskell}
    (\x -> 4 * x) . (\y -> 3 + y)
  = \x -> 4 * (3 + x)
\end{minted}


\section*{Aufgabe 3.3}
\paragraph{1)}
\begin{minted}{haskell}
    \(f, g) p x -> if p x then f x else g x
 :: ((a -> b), (a -> b)) -> (a -> Bool) -> a -> b
\end{minted}

\paragraph{2)}
\begin{minted}{haskell}
    (curry (\(x, y) -> if x < y then y else x)) 3
 :: Int -> Int
\end{minted}


\section*{Aufgabe 3.4}
\inputminted{haskell}{update.hs}

\end{document}
